---
layout: post
title: Generative Models
date: 2025-02-15 21:10 +0800
categories: [Fundamentals]
tags: [generative models, discriminative models, bayes' theorem]
pin: true
math: true
mermaid: true
---


## Introduction of Generative Models [[1]](#references)

When discussing **generative models**, it's essential to understand how machine learning approaches tasks. Consider a scenario where we aim to distinguish between elephants and dogs, there are primarily two modeling approaches: discriminative and generative:

1. **Discriminative Modeling:** This approach involves building a model that directly predicts **classification labels** or identifies the **decision boundary** between elephants and dogs.
2. **Generative Modeling:** This approach entails constructing separate models for elephants and dogs, capturing their **respective characteristics**. A new animal is then compared against each model to determine which it resembles more closely.

In discriminative modeling, the focus is on learning the conditional probability of labels given the input data, denoted as 
$$p(y|{x})$$. Techniques like logistic regression exemplify this by modeling the probability of a label based on input features. Alternatively, methods such as the perceptron algorithm aim to find a decision boundary that maps new observations to specific labels $$\{0,1\}$$, such as $$0$$ for dogs and $$1$$ for elephants.

Conversely, generative modeling focuses on understanding how the data is generated by learning the joint probability distribution $$p(x,y)$$ or the likelihood 
$$p(x|{y})$$ along with the prior probability $$p(y)$$. This approach models the distribution of the input data for each class, enabling the generation of new data points and facilitating classification by applying Bayes' theorem to compute the posterior probability:

$$ 
p(y|x) = \frac{p(x|y)p(y)}{p(x)}
$$

The denominator $$p(x)$$ is the marginal probability that sums the joint probability $$p(x,y)$$ over all possible labels $$y$$:

$$
\begin{aligned}
p(x) &= \sum_{y} p(x,y) \\
     &= \sum_{y} p(x|y)p(y) \\
     &= p(x|y=0)p(y=0) + p(x|y=1)p(y=1)
\end{aligned}
$$

Actually $$p(x)$$ acts as a **normalization constant** as it does not depend on the label $$y$$. To be more specific, $$p(x)$$ does not change no matter how $$y$$ varies. So when calculating 
$$p(y|x)$$, we do not need to compute $$p(x)$$:

$$
\begin{aligned}
\arg\max_y p(y|x) &= \arg\max_y \frac{p(x|y)p(y)}{p(x)}\\
&= \arg\max_y p(x|y)p(y) \\
\end{aligned}
$$

Let's consider a new task of spam classification. $$ x^{(i)} $$ is the feature vector of the $$i$$-th email, and $$ y^{(i)} $$ is the label indicating whether the email is spam ($$1$$) or not-spam ($$0$$). Following examples show how discriminative and generative models approach the same problem differently.

### Example 1: Logistic Regression as a Discriminative Model

Since it is a binary classification problem, it makes sense to choose a hypothesis $$h_{\theta}(x)$$ that ranges in $$(0,1)$$ to represent the probability of 
$$p(y=1|x)$$, where 
$$p(y=0|x) = 1 - h_{\theta}(x)$$. Then we can set the threshold of $$h_{\theta}(x)$$ to be $$0.5$$ to predict if an email is spam. Logistic function fits this case well as it ranges in $$(0,1)$$ for $$z\in(-\infty, +\infty)$$:

$$
h_{\theta}(x) = g(\theta^T x) = \frac{1}{1 + e^{-\theta^T x}}
$$

where 

$$
g(z) = \frac{1}{1 + e^{-z}} 
$$ 

is called the logistic function or sigmoid function. Below is a plot of the sigmoid function:

![Sigmoid Function](/assets/img/posts/sigmoid.png){: width="300" height="250" }

From the plot, we can see $$g(z)$$ tends to $$0$$ as $$z\to-\infty$$ and tends to $$1$$ as $$z\to+\infty$$. When $$z=0$$, $$g(z)=0.5$$. $$g(z)$$ or $$h_{\theta}(x)$$ is always bounded between $$0$$ and $$1$$. To keep the convention of letting $$x_0=1$$, we can rewrite the expression of $$z$$ in the hypothesis as $$z = \theta^T x = \theta_0 + \sum_{j=1}^n \theta_j x_j$$, where $$\theta_0$$ is the bias term and $$\theta_j$$ is the weight of the $$j$$-th feature $$x_j$$. Please note that other functions that smoothly and monotonically increase from $$0$$ to $$1$$ can be also considered for $$h_{\theta}(x)$$.

Now we can continue to use the maximum likelihood estimation to find the best parameters $$\theta$$ for logistic regression model. To indicate $$\theta$$ as the parameter vector in the conditional probability distribution 
$$p(y|x)$$, we can rewrite the expression of $$p(y|x)$$ as:

$$
\begin{aligned}
p(y=1|x;\theta) &= h_{\theta}(x) \\
p(y=0|x;\theta) &= 1 - h_{\theta}(x) \\
p(y|x;\theta) &= (h_{\theta}(x))^y (1-h_{\theta}(x))^{1-y}
\end{aligned}
$$

Assume that n training examples are drawn independently from the same distribution, we can write the likelihood function of parameter $$\theta$$ as:

$$
\begin{aligned}
L(\theta) &= p(\vec{y}|X;\theta) \\
&= p(y^{(1)},y^{(2)},...,y^{(n)}|x^{(1)},x^{(2)},...,x^{(n)};\theta) \\
&= \prod_{i=1}^n p(y^{(i)}|x^{(i)};\theta) \\
&= \prod_{i=1}^n (h_{\theta}(x^{(i)}))^{y^{(i)}}(1-h_{\theta}(x^{(i)}))^{1-y^{(i)}} \\
\end{aligned}
$$

Since it is easier to work with the log-likelihood function to maximize, we can take the logarithm of the likelihood function:

$$
\begin{aligned}
\ell(\theta) = \log{L}(\theta) &= \log\prod_{i=1}^n (h_{\theta}(x^{(i)}))^{y^{(i)}}(1-h_{\theta}(x^{(i)}))^{1-y^{(i)}} \\
&= \sum_{i=1}^n y^{(i)}\log h_{\theta}(x^{(i)}) + \sum_{i=1}^n (1-y^{(i)})\log(1-h_{\theta}(x^{(i)})) \\
&= \left[\begin{array}{cccc}
  y^{(1)} & y^{(2)} & \cdots & y^{(n)}  \\
\end{array}\right]log
\begin{bmatrix}
  g(\theta^T x^{(1)})  \\
  g(\theta^T x^{(2)}) \\
  \vdots \\
  g(\theta^T x^{(n)})
\end{bmatrix} + 
\left[\begin{array}{cccc}
  1-y^{(1)} & 1-y^{(2)} & \cdots & 1-y^{(n)}  \\
\end{array}\right]log
\begin{bmatrix}
  (1-g(\theta^T x^{(1)}))  \\
  (1-g(\theta^T x^{(2)})) \\
  \vdots \\
  (1-g(\theta^T x^{(n)}))
\end{bmatrix} \\
&= y^T\log{g(X\theta)} + (1-y)^T\log{(1-g(X\theta))}
\end{aligned}
$$

As we choose sigmoid function $$g(z)$$ to represent the hypothesis $$h_{\theta}(x)$$, let's firstly compute the derivative of $$g(z)$$ with respect to $$z$$:

$$
\begin{aligned}
g^\prime(z) &= \frac{d}{dz}\frac{1}{1+e^{-z}} \\
&= \frac{-1}{(1+e^{-z})^2}\frac{d}{dz}(1+e^{-z}) = \frac{-1}{(1+e^{-z})^2}(-e^{-z}) \\
&= \frac{e^{-z}}{(1+e^{-z})^2} = \frac{1}{(1+e^{-z})}(1-\frac{1}{1+e^{-z}}) \\
&= g(z)(1-g(z))
\end{aligned}
$$

Then apply the chain rule to compute the derivative of $$\ell(\theta)$$ with respect to $$\theta$$. To make it simple, we only consider the derivative of $$\ell(\theta)$$ with respect to $$\theta_j$$ and for each training example $$x^{(i)}$$ and label $$y^{(i)}$$. As we only use sample $$i$$ to compute the derivative we can drop the index $$i$$ for convenience:

$$
\begin{aligned}
\frac{\partial}{\partial \theta_j} \ell(\theta) &= \left(y\frac{1}{g(\theta^T{x})} - (1-y)\frac{1}{1-g(\theta^T{x})}\right)\frac{\partial}{\partial \theta_j}g(\theta^T{x}) \\
&= \left(y\frac{1}{g(\theta^T{x})} - (1-y)\frac{1}{1-g(\theta^T{x})}\right)g(\theta^T{x})(1-g(\theta^T{x}))\frac{\partial}{\partial \theta_j}\theta^T{x} \\
&= \left(y\frac{1}{g(\theta^T{x})} - (1-y)\frac{1}{1-g(\theta^T{x})}\right)g(\theta^T{x})(1-g(\theta^T{x}))x_j \\
&= \left(y(1-g(\theta^T{x})) - (1-y)g(\theta^T{x})\right)x_j \\
&= (y-h_{\theta}(x))x_j
\end{aligned}
$$

Therefore gives us the stochastic gradient ascent rule, where $$(y^{(i)}-h_{\theta}(x^{(i)}))x_j^{(i)}$$ is the gradient of the log-likelihood function with respect to the $$i$$-th training example:

$$
\theta_j := \theta_j + \alpha(y^{(i)}-h_{\theta}(x^{(i)}))x_j^{(i)}
$$




### Example 2: Gaussian Discriminant Analysis as a Generative Model

Let's say the feature vector $$x$$ of an email is using TF-IDF[[2]](#references) that measures the importance of words in the email. TF-IDF (Term Frequency-Inverse Document Frequency) is a numerical statistic that reflects the importance of a word in a document relative to a collection of documents (corpus). It is calculated as:

$$
\text{TF-IDF}(t, d) = \text{TF}(t, d) \times \text{IDF}(t)
$$

where:

$$
\begin{aligned}
\text{TF}(t, d) &= \frac{\text{Number of times term } t \text{ appears in document } d}{\text{Total number of terms in document } d} \\
\text{IDF}(t) &= \log\left(\frac{\text{Total number of documents}}{\text{Number of documents containing term } t}\right)
\end{aligned}
$$

As TF-IDF is continuous we can model 
$$p(x|y)$$ as a multivariate normal distribution. Then the model can be represented as:

$$
\begin{aligned}
y &\sim \text{Bernoulli}(\phi) \\
x|y=0 &\sim \mathcal{N}(\mu_0, \Sigma) \\
x|y=1 &\sim \mathcal{N}(\mu_1, \Sigma)
\end{aligned}
$$

Writing out the distributions, we have:

$$
\begin{aligned}
p(y) &= \phi^y(1-\phi)^{1-y} \\
p(x|y=0) &= \frac{1}{(2\pi)^{n/2}|\Sigma|^{1/2}}exp\left(-\frac{1}{2}(x-\mu_0)^T\Sigma^{-1}(x-\mu_0)\right) \\
p(x|y=1) &= \frac{1}{(2\pi)^{n/2}|\Sigma|^{1/2}}exp\left(-\frac{1}{2}(x-\mu_1)^T\Sigma^{-1}(x-\mu_1)\right) \\
\end{aligned}
$$













## References

[1] Ng, Andrew. "[CS229: Machine Learning Course Notes](https://cs229.stanford.edu/main_notes.pdf)". Stanford University, 2018.
[2] Manning, Christopher D., et al. "[Introduction to Information Retrieval](https://nlp.stanford.edu/IR-book/pdf/irbookprint.pdf)". Stanford University, 2009.


